prove asm_inj_drop & remove admits in LowerBound

x86/LowerBound.v
@@ -5,7 +5,7 @@ Require Import Locations Stacklayout Conventions Linking.
 Require Export Asm.
 Require Import Simulation Memory ValuesC.
 Require Import Skeleton ModSem Mod sflib StoreArguments AsmC Sem Syntax LinkingC Program SemProps.
-Require Import GlobalenvsC MemoryC2 LowerBoundExtra Lia LinkingC2 mktac MemdataC LocationsC.
+Require Import GlobalenvsC MemoryC2 LowerBoundExtra Lia LinkingC2 mktac MemdataC LocationsC AsmExtra.
 
 Set Implicit Arguments.
 
@@ -91,6 +91,11 @@ Section PRESERVATION.
     ss.
   Qed.
 
+  Let ININCL: forall p (IN: In p prog), <<INCL: SkEnv.includes skenv_link p.(Mod.sk)>>.
+  Proof.
+    eapply link_includes; et.
+  Qed.
+
   Definition local_genv (p : Asm.program) :=
     (skenv_link.(SkEnv.project) p.(Sk.of_program fn_sig)).(SkEnv.revive) p.
 
@@ -119,7 +124,8 @@ Section PRESERVATION.
   Qed.
 
   Definition genv_le (ge_src ge_tgt: Genv.t fundef unit): Prop :=
-    sub_match_genvs eq ge_src ge_tgt.
+    (* sub_match_genvs eq ge_src ge_tgt. *)
+    sub_match_genvs (@def_match _ _) ge_src ge_tgt.
 
   Inductive skenv_inject {F V} (ge: Genv.t F V) (j: meminj): Prop :=
   | sken_inject_intro
@@ -178,7 +184,7 @@ Section PRESERVATION.
   Lemma sub_match_local_genv ge_local
         (MATCHGE: genv_le ge_local tge)
     :
-      sub_match_genvs (fun fdef skdef => skdef_of_gdef fn_sig fdef = skdef) ge_local skenv_link.
+      sub_match_genvs (fun fdef skdef => def_match (skdef_of_gdef fn_sig fdef) (skdef)) ge_local skenv_link.
   Proof.
     destruct match_skenv_link_tge. inv MATCHGE.
     unfold Genv.find_symbol, Genv.find_def in *. econs.
@@ -189,6 +195,7 @@ Section PRESERVATION.
       specialize (mge_defs b). inv mge_defs.
       + eq_closure_tac.
       + eq_closure_tac. esplits; eauto.
+        inv MATCHDEF; ss; des_ifs; econs.
   Qed.
 
   Inductive valid_owner fptr (p: Asm.program) : Prop :=
@@ -196,27 +203,18 @@ Section PRESERVATION.
       fd
       (MSFIND: ge.(Ge.find_fptr_owner) fptr (AsmC.modsem skenv_link p))
       (FINDF: Genv.find_funct (local_genv p) fptr = Some (Internal fd))
-      (SIZEWF: 4 * size_arguments (fn_sig fd) <= Ptrofs.max_unsigned).
+      (SIZEWF: 4 * size_arguments (fn_sig fd) <= Ptrofs.max_unsigned)
+      (PROGIN: In (AsmC.module p) prog)
+  .
 
-  Inductive _genv_le : forall A:Type, A -> Genv.t fundef unit -> Prop :=
-  | _genv_le_intro
-      ge1 ge2
-      (LE: genv_le ge1 ge2)
+  Lemma owner_genv_le p
+      (IN: In (AsmC.module p) prog)
     :
-      _genv_le ge1 ge2.
-
-  Lemma owner_genv_le ms
-        (IN: In ms (fst ge))
-    :
-      _genv_le ms.(ModSem.globalenv) tge.
+      genv_le (local_genv p) tge.
   Proof.
-    unfold ge in *. ss. des.
-    { admit "".
-    }
+    unfold ge in *.
     unfold load_modsems, flip, Mod.modsem, skenv_link, Sk.load_skenv, prog in *. ss.
-    rewrite list_map_compose in IN. ss.
-    eapply in_map_iff in IN. des. clarify. unfold modsem. ss. econs.
-
+    eapply in_map_iff in IN. des. clarify. apply inj_pair2 in H0. destruct H0. unfold local_genv.
     assert(INCL: SkEnv.includes (Genv.globalenv sk) (Sk.of_program fn_sig x)).
     { exploit link_includes; et.
       { rewrite in_map_iff. esplits; et. }
@@ -251,10 +249,7 @@ Section PRESERVATION.
         i; des.
         ss. congruence.
 
-    - exists d0. splits; eauto.
-
-      dup FIND. unfold SkEnv.revive in FIND.
-
+    - dup FIND. unfold SkEnv.revive in FIND.
       eapply Genv_map_defs_def in FIND. des.
       gesimpl.
 
@@ -275,39 +270,31 @@ Section PRESERVATION.
       assert(i = i0).
       { apply Genv.find_invert_symbol in TMP0. unfold skenv_link in EQ. clarify. }
       clarify.
-      assert(TP: (prog_defmap tprog) ! i0 = Some d0).
-      { rename x into xx.
-        hexploit (link_list_linkorder _ LINK); et. intro LO; des. rewrite Forall_forall in *.
-        specialize (LO xx IN0).
-        Local Transparent Linker_prog.
-        ss.
-        Local Opaque Linker_prog.
-        des.
-        exploit LO1; et. i; des.
-        rewrite H.
-        assert(INT: ~ASTC.is_external d0).
-        { ss. }
-        clear - INT H0.
-        inv H0; ss.
-        - inv H; ss.
-        - inv H; ss. destruct info1, info2; ss. inv H1; ss.
-          + admit "this does not hold!".
-          + admit "this does not hold!".
-      }
-      apply Genv.find_def_symbol in TP. des.
-      assert(b0 = b).
-      { apply Genv.invert_find_symbol in EQ. uge. rewrite mge_symb in TP. unfold skenv_link in EQ. clarify. }
-      clarify.
-  Qed.
 
-  Lemma valid_owner_genv_le fptr p
-        (OWNER: valid_owner fptr p)
-    :
-      genv_le (local_genv p) tge.
-  Proof.
-    inv OWNER. inv MSFIND.
-    eapply owner_genv_le in MODSEM. inv MODSEM.
-    unfold genv in H. eapply inj_pair2 in H. clarify.
+      hexploit (link_list_linkorder _ LINK); et. intro LO; des. rewrite Forall_forall in *.
+      specialize (LO x IN0).
+      Local Transparent Linker_prog.
+      ss.
+      Local Opaque Linker_prog.
+      des.
+      exploit LO1; et. i; des.
+      assert(INT: ~ASTC.is_external d0).
+      { ss. }
+      assert(INT0: ~ASTC.is_external gd2).
+      { Local Transparent Linker_def. inv H0.
+        - inv H2.
+          + ss.
+          + ss.
+        - inv H2; ss.
+      }
+      exists gd2. splits; eauto.
+      + apply Genv.find_def_symbol in H. des.
+        assert(b0 = b).
+        { apply Genv.invert_find_symbol in EQ. uge. rewrite mge_symb in H. unfold skenv_link in EQ. clarify. }
+        clarify.
+      + inv H0; ss.
+        * inv H2; ss.
+        * inv H2; ss. destruct info1, info2. econs.
   Qed.
 
   Lemma symb_preserved id
@@ -351,7 +338,7 @@ Section PRESERVATION.
     cinv (mge_defs b).
     - rewrite Heq in *. clarify.
     - rewrite Heq in *. clarify.
-      unfold skdef_of_gdef, fundef in *. rewrite FIND in *. des_ifs.
+      unfold skdef_of_gdef, fundef in *. rewrite FIND in *. inv MATCHDEF. des_ifs.
   Qed.
 
 (** ********************* initial memory *********************************)
@@ -384,9 +371,6 @@ Section PRESERVATION.
       unfold skenv_link, Sk.load_skenv in *. des_ifs.
     - des_ifs.
   Qed.
-
-  Definition agree (j: meminj) (rs_src rs_tgt: regset) : Prop :=
-    forall pr, Val.inject j (rs_src pr) (rs_tgt pr).
 
   Lemma system_symbols_inject j
         (SKINJ: skenv_inject skenv_link j)
@@ -443,7 +427,6 @@ Section PRESERVATION.
     :
       symbols_inject j (System.globalenv skenv_link) skenv_link.
   Proof.
-
     destruct match_skenv_link_tge. inv SKINJ.
     unfold System.globalenv.
     rr. esplits; ss.
@@ -451,6 +434,56 @@ Section PRESERVATION.
       exploit DOMAIN; et. i; clarify.
     - i. exploit Genv.genv_symb_range; eauto.
   Qed.
+
+  (* Lemma local_genv_symbols_inject p j *)
+  (*       (SKINJ: skenv_inject skenv_link j) *)
+  (*       (IN: In (AsmC.module p) prog) *)
+  (*   : *)
+  (*     symbols_inject j (local_genv p) tge. *)
+  (* Proof. *)
+  (* Admitted. *)
+  (*   inv SKINJ. *)
+  (*   exploit owner_genv_le; eauto. intros GELE. *)
+  (*   generalize match_skenv_link_tge. intros MATCH. *)
+  (*   inv MATCH. *)
+  (*   exploit SkEnv.project_impl_spec; eauto. *)
+  (*   { eapply ININCL; eauto. } *)
+  (*   intros PROJECT. inv PROJECT. *)
+
+  (*   econs; esplits; ss; i. *)
+  (*   - unfold local_genv in *. unfold SkEnv.revive, Genv.public_symbol. ss. *)
+  (*     rewrite Genv_map_defs_symb. ss. *)
+  (*     rewrite genv_public_eq in *. *)
+  (*     unfold Genv.find_symbol, proj_sumbool in *. *)
+  (*     erewrite mge_symb. *)
+  (*     des_ifs; exfalso. *)
+  (*     + erewrite SYMBKEEP in Heq0; eauto. clarify. *)
+  (*     + erewrite SYMBKEEP in Heq0; eauto. clarify. *)
+
+  (*   - unfold local_genv in *. *)
+  (*     unfold SkEnv.revive, Genv.public_symbol in H0. *)
+  (*     rewrite Genv_map_defs_symb in H0. *)
+  (*     erewrite SYMBKEEP in H0. *)
+  (*     + unfold Genv.find_symbol in *. rewrite mge_symb in *. *)
+  (*       exploit DOMAIN. *)
+  (*       { instantiate (1:=b1). *)
+  (*         exploit Genv.genv_symb_range; eauto. } *)
+  (*       i. clarify. *)
+  (*     + apply NNPP. ii. exploit SYMBDROP. *)
+  (*       { instantiate (1:=id). tauto. } *)
+  (*       i. congruence. *)
+
+  (*   - unfold local_genv in *. *)
+  (*     unfold SkEnv.revive, Genv.public_symbol, proj_sumbool in *. *)
+  (*     rewrite Genv_map_defs_symb in *. ss. des_ifs. *)
+  (*     erewrite SYMBKEEP in Heq; eauto. *)
+  (*     unfold Genv.find_symbol in *. *)
+  (*     rewrite mge_symb. esplits; eauto. *)
+  (*     exploit DOMAIN; eauto. *)
+  (*     exploit Genv.genv_symb_range; eauto. *)
+
+  (*   - admit "doesn't hold". *)
+  (* Qed. *)
 
   Lemma external_function_sig
         v skd ef
@@ -551,48 +584,53 @@ Section PRESERVATION.
     Proof.
     Admitted.
 
-    Lemma asm_step_preserve_injection
-          rs_src0 rs_src1 m_src0 m_src1 tr j0
-          rs_tgt0 m_tgt0
-          ge_src ge_tgt
-          (GENVLE: genv_le ge_src ge_tgt)
-          (DOMAIN: forall b (LT: Plt b ge_src.(Genv.genv_next)),
-              j0 b = Some(b, 0))
-          (NOEXTFUN: no_extern_fun ge_src)
-          (AGREE: agree j0 rs_src0 rs_tgt0)
-          (INJ: Mem.inject j0 m_src0 m_tgt0)
-          (STEP: Asm.step skenv_link ge_src (Asm.State rs_src0 m_src0) tr (Asm.State rs_src1 m_src1))
-      :
-        exists rs_tgt1 m_tgt1 j1,
-          (Asm.step skenv_link ge_tgt (Asm.State rs_tgt0 m_tgt0) tr (Asm.State rs_tgt1 m_tgt1)) /\
-          (agree j1 rs_src1 rs_tgt1) /\
-          (Mem.inject j1 m_src1 m_tgt1) /\
-          (inject_incr j0 j1) /\
-          (inject_separated j0 j1 m_src0 m_tgt0)
-    .
-    Proof.
-    Admitted.
+(* <<<<<<< HEAD *)
+(*     Lemma asm_step_preserve_injection *)
+(*           rs_src0 rs_src1 m_src0 m_src1 tr j0 *)
+(*           rs_tgt0 m_tgt0 *)
+(*           ge_src ge_tgt *)
+(*           (GENVLE: genv_le ge_src ge_tgt) *)
+(*           (DOMAIN: forall b (LT: Plt b ge_src.(Genv.genv_next)), *)
+(*               j0 b = Some(b, 0)) *)
+(*           (NOEXTFUN: no_extern_fun ge_src) *)
+(*           (AGREE: agree j0 rs_src0 rs_tgt0) *)
+(*           (INJ: Mem.inject j0 m_src0 m_tgt0) *)
+(*           (STEP: Asm.step skenv_link ge_src (Asm.State rs_src0 m_src0) tr (Asm.State rs_src1 m_src1)) *)
+(*       : *)
+(*         exists rs_tgt1 m_tgt1 j1, *)
+(*           (Asm.step skenv_link ge_tgt (Asm.State rs_tgt0 m_tgt0) tr (Asm.State rs_tgt1 m_tgt1)) /\ *)
+(*           (agree j1 rs_src1 rs_tgt1) /\ *)
+(*           (Mem.inject j1 m_src1 m_tgt1) /\ *)
+(*           (inject_incr j0 j1) /\ *)
+(*           (inject_separated j0 j1 m_src0 m_tgt0) *)
+(*     . *)
+(*     Proof. *)
+(*     Admitted. *)
 
-    Lemma asm_step_max_perm ge_src rs0 rs1 m0 m1 tr
-          (STEP: Asm.step skenv_link ge_src (Asm.State rs0 m0) tr (Asm.State rs1 m1))
-          b ofs p
-          (VALID: Mem.valid_block m0 b)
-          (PERM: Mem.perm m1 b ofs Max p)
-      :
-        Mem.perm m0 b ofs Max p.
-    Proof.
-    Admitted.
+(*     Lemma asm_step_max_perm ge_src rs0 rs1 m0 m1 tr *)
+(*           (STEP: Asm.step skenv_link ge_src (Asm.State rs0 m0) tr (Asm.State rs1 m1)) *)
+(*           b ofs p *)
+(*           (VALID: Mem.valid_block m0 b) *)
+(*           (PERM: Mem.perm m1 b ofs Max p) *)
+(*       : *)
+(*         Mem.perm m0 b ofs Max p. *)
+(*     Proof. *)
+(*     Admitted. *)
+
+(* ======= *)
+(* >>>>>>> prove asm_inj_drop & remove admits in LowerBound *)
 
   End ASMLEMMAS.
 
   Lemma local_genv_no_extern_fun p :
-    no_extern_fun (local_genv p).
+    forall (IN: In (AsmC.module p) prog),
+      no_extern_fun (local_genv p).
   Proof.
     unfold no_extern_fun. ii. unfold local_genv in *. des.
     unfold Genv.find_funct_ptr in *. des_ifs.
     exploit SkEnv.project_revive_no_external; eauto.
     { ss. destruct ef; ss. }
-    admit "INCL".
+    exploit ININCL; eauto.
   Qed.
 
   Lemma ALLOC_NEXT_INCR F V (gen: Genv.t F V) x m0 m1
@@ -808,7 +846,8 @@ Section PRESERVATION.
       (FRAME: fr = Frame.mk (AsmC.modsem skenv_link p) (AsmC.mkstate init_rs1 st))
       (STACK: match_stack j P0 init_rs1 frs)
       (WF: wf_init_rs j st.(st_rs) init_rs0)
-      (IN: genv_le (local_genv p) tge)
+      (GELE: genv_le (local_genv p) tge)
+      (PROGIN: In (AsmC.module p) prog)
       (SIG: exists skd, skenv_link.(Genv.find_funct) (init_rs0 # PC)
                         = Some skd /\ SkEnv.get_sig skd = sg)
       (RSPPTR: st.(st_rs) # RSP = Vptr blk ofs true)
@@ -833,7 +872,8 @@ Section PRESERVATION.
       (INITRS: init_rs0 = st.(st_rs))
       (STACK: match_stack j P0 init_rs1 frs)
       (MEM: m = st.(st_m))
-      (IN: genv_le (local_genv p) tge)
+      (GELE: genv_le (local_genv p) tge)
+      (PROGIN: In (AsmC.module p) prog)
       (SIG: exists skd, skenv_link.(Genv.find_funct) (init_rs0 # PC)
                         = Some skd /\ SkEnv.get_sig skd = sg)
       (RSPPTR: init_rs0 # RSP = Vptr blk ofs true)
@@ -1076,6 +1116,7 @@ Section PRESERVATION.
       (AGREE: agree j rs_src rs_tgt)
       (INJ: Mem.inject j m_src m_tgt)
       (GELE: genv_le (local_genv p) tge)
+      (PROGIN: In (AsmC.module p) prog)
       (GEINJECT: skenv_inject skenv_link j)
       (FRAME: fr = Frame.mk (AsmC.modsem skenv_link p)
                             (AsmC.mkstate init_rs (Asm.State rs_src m_src)))
@@ -1164,7 +1205,8 @@ Section PRESERVATION.
     inv FINAL0. clarify. inv STACK. econs.
     - specialize (AGREE PC). rewrite RSRA in *. rewrite RSRA0 in *.
       inv AGREE; ss.
-    - des. rewrite RSPC in *. exploit local_global_consistent; eauto. intro SGEQ. rewrite <- SGEQ in *. clarify.
+    - des. rewrite RSPC in *. exploit local_global_consistent; eauto.
+      intro SGEQ. rewrite <- SGEQ in *. clarify.
       ss. unfold signature_main, loc_arguments, loc_result in *.
       Transparent Archi.ptr64. ss. unfold loc_result_64 in *. ss. clarify.
       ss. specialize (AGREE RAX). rewrite INT in *. inv AGREE; auto.
@@ -1198,6 +1240,7 @@ Section PRESERVATION.
   Lemma asm_step_internal_simulation
         st_src0 st_src1 st_tgt0 tr frs p init_rs n0
         (STEP: Asm.step skenv_link (local_genv p) st_src0 tr st_src1)
+        (PROGIN: In (AsmC.module p) prog)
         (MTCHST: match_states (State ((Frame.mk (AsmC.modsem skenv_link p)
                                                 (AsmC.mkstate init_rs st_src0))::frs))
                               st_tgt0 n0)
@@ -1208,21 +1251,39 @@ Section PRESERVATION.
                                        (AsmC.mkstate init_rs st_src1))::frs))
                      st_tgt1 n1.
   Proof.
-    inv MTCHST. dup FRAME. apply asm_frame_inj in FRAME0.
+    inv MTCHST. dup FRAME. dup FRAME.
+    apply asm_frame_inj in FRAME0.
     apply asm_frame_inj2 in FRAME. inv FRAME0. destruct st_src1.
-    rewrite <- FRAME in GELE.
-    exploit asm_step_preserve_injection; eauto.
-    - inv GEINJECT. i. eapply DOMAIN.
-      eapply sub_mge_next in GELE. destruct match_skenv_link_tge.
-      rewrite <- mge_next. eapply Plt_Ple_trans; eauto.
-    - eapply local_genv_no_extern_fun.
-    - ii. des. esplits; eauto; econs; eauto.
+    eapply owner_genv_le in PROGIN.
+    rewrite FRAME in *.
+
+    exploit AsmExtra.asm_step_preserve_injection; eauto.
+
+    { clear FRAME1 FRAME. i. inv GELE. inv GEINJECT.
+      exploit sub_mge_defs0; eauto. i. des.
+      inv WFSKELINK.
+      exploit DOMAIN.
+      - erewrite <- Genv.mge_next; try apply match_skenv_link_tge.
+        instantiate (1:= b_src).
+        exploit Genv.genv_defs_range; eauto.
+      - i. clarify. esplits; eauto.
+    }
+
+    { i. inv GELE. inv GEINJECT.
+      exploit sub_mge_symb0; eauto. i. esplits; eauto.
+      exploit DOMAIN; eauto.
+      erewrite <- Genv.mge_next; try apply match_skenv_link_tge.
+      exploit Genv.genv_symb_range; eauto.
+    }
+
+    { eapply system_symbols_inject; eauto. }
+
+    - ii. des. rewrite <- senv_same in *. esplits; eauto. econs; eauto.
       +
         {
-          clear - INJ H2 H3 GEINJECT.
           inv GEINJECT. econs.
           - i. unfold inject_incr in *.
-            eapply H2. eapply DOMAIN. eauto.
+            eapply INCR. eapply DOMAIN. eauto.
           - i. ss.
             destruct (Genv.block_is_volatile skenv_link b2) eqn:EQ1;
             destruct (Genv.block_is_volatile skenv_link b1) eqn:EQ2;
@@ -1230,13 +1291,26 @@ Section PRESERVATION.
 
             + set (Genv.block_is_volatile_below _ _ EQ1).
               destruct (j b1) eqn : EQ.
-              * destruct p0. apply H2 in EQ. clarify.
-              * exfalso. eapply H3 in EQ. specialize (EQ INJ0). des.
+              * destruct p2. apply INCR in EQ. clarify.
+              * exfalso. eapply SEP in EQ. specialize (EQ INJ1). des.
                 inv INJ. unfold Mem.valid_block in *. eauto.
             + eapply Genv.block_is_volatile_below in EQ2.
               set (DOMAIN _ EQ2).
-              set (H2 _ _ _ e). clarify. auto.
+              set (INCR _ _ _ e). clarify. auto.
         }
+      + instantiate (1:=init_rs0).
+        assert (JEQ: @JMeq
+                       (ModSem.state (modsem skenv_link p))
+                       {| init_rs := init_rs0; st := Asm.State r m |}
+                       (ModSem.state (modsem skenv_link p0))
+                       {| init_rs := init_rs0; st := Asm.State r m |}).
+        { econs. }
+        revert JEQ.
+        generalize ({| init_rs := init_rs0; st := Asm.State r m |} : ModSem.state (modsem skenv_link p0)) at 2 4.
+        generalize ({| init_rs := init_rs0; st := Asm.State r m |} : ModSem.state (modsem skenv_link p)).
+        apply f_equal with (f:=Frame.ms) in FRAME1. simpl in FRAME1.
+        clear - FRAME1. destruct FRAME1.
+        ii. f_equal. apply JMeq_eq. eauto.
       + eapply match_stack_incr; eauto.
       + eapply inj_range_wf_step; cycle 2; eauto.
         i. destruct (j blk) eqn: EQ; eauto. destruct p2. left.
@@ -1283,9 +1357,11 @@ Section PRESERVATION.
     - eapply callee_save_agree; eauto.
       etrans; eauto.
     - eauto.
-    - eapply IN.
+    - eapply GELE0.
     - ss.
-    - unfold Frame.update_st. s. repeat f_equal. eapply local_global_consistent; try apply GELE; eauto.
+    - ss.
+    - unfold Frame.update_st. s. repeat f_equal.
+      eapply local_global_consistent; try eapply GELE; eauto.
     - eapply match_stack_incr; [eauto| | eauto]. instantiate (1:=P). eauto.
     - auto.
     - des_ifs.
@@ -1352,13 +1428,15 @@ Section PRESERVATION.
         args frs st_tgt p n
         (MTCHST: match_states (Callstate args frs) st_tgt n)
         (OWNER: valid_owner args.(Args.fptr) p)
+        (PROGIN: In (AsmC.module p) prog)
     :
       exists rs m,
         (AsmC.initial_frame skenv_link p args (AsmC.mkstate rs (Asm.State rs m))) /\
         (match_states (State ((Frame.mk (AsmC.modsem skenv_link p) (AsmC.mkstate rs (Asm.State rs m))) :: frs)) st_tgt 0).
   Proof.
-    inv MTCHST. dup OWNER. apply valid_owner_genv_le in OWNER0.
-    inv OWNER. des. ss.
+    inv MTCHST. dup OWNER. inv OWNER.
+    exploit owner_genv_le; eauto. intros GELE.
+    des. ss.
     set (nextblock_unvalid := nextblock_unvalid INJECT).
     destruct (Mem.alloc args.(Args.m) 0 (4 * size_arguments (fn_sig fd))) eqn:MEQ.
     assert (Genv.find_funct skenv_link (Args.fptr args) =
@@ -1367,7 +1445,9 @@ Section PRESERVATION.
       unfold Genv.find_funct, Genv.find_funct_ptr in *.
       exploit sub_match_local_genv; eauto. intros MATCHGE.
       set (sub_mge_defs MATCHGE).
-      des_ifs. specialize (e _ _ Heq1). des; clarify. }
+      des_ifs. specialize (e _ _ Heq1). des; clarify.
+      inv MATCHDEF. ss.
+    }
     clarify. ss.
 
     exists (arg_copy_reg (fn_sig fd) (Args.vs args)
@@ -1419,7 +1499,8 @@ Section PRESERVATION.
         eapply Mem.extends_inject_compose.
         * eapply arg_copy_mem_extends.
         * eapply memcpy_inject; eauto.
-      + eapply valid_owner_genv_le. econs; eauto.
+      + eauto.
+      + ss.
       + unfold callee_injection. inv GEINJECT. econs; i.
         { des_ifs; eauto. exploit (DOMAIN b); auto. i. clarify. }
         des_ifs; [| eauto].
@@ -1474,6 +1555,7 @@ Section PRESERVATION.
         args frs st_tgt p n
         (MTCHST: match_states (Callstate args frs) st_tgt n)
         (OWNER: valid_owner args.(Args.fptr) p)
+        (PROGIN: In (AsmC.module p) prog)
     :
       exists st_src,
         step ge (Callstate args frs) E0 st_src /\ match_states st_src st_tgt 0.
@@ -1524,7 +1606,7 @@ Section PRESERVATION.
   Lemma owner_asm_or_system fptr ms
         (OWNER: Ge.find_fptr_owner ge fptr ms)
     :
-      (<<ASMMOD: exists p, ms= AsmC.modsem skenv_link p >>)\/
+      (<<ASMMOD: exists p, ms = AsmC.modsem skenv_link p /\ In (AsmC.module p) prog>>)\/
       (<<SYSMOD: ms = System.modsem skenv_link>>).
   Proof.
     inv OWNER. clear - MODSEM. unfold ge in *.
@@ -1532,6 +1614,10 @@ Section PRESERVATION.
     ss. des; auto.
     left. generalize progs ms MODSEM.
     intros l. induction l; ss; i. des; eauto.
+    rewrite in_map_iff in *. des. clarify.
+    rewrite in_map_iff in *. des. clarify.
+    exists x1.
+    esplits; eauto. right. apply in_map_iff. esplits; et.
   Qed.
 
   Lemma find_fptr_owner_determ
@@ -1555,23 +1641,27 @@ Section PRESERVATION.
                       fptr (System.modsem skenv_link)>>) \/
       (<<UNSAFE: ~ safe (sem prog) st>>).
   Proof.
-    destruct (classic (exists ms, Ge.find_fptr_owner ge args.(Args.fptr) ms)) as [[ms OWNER] | NOOWNER].
-    - destruct (owner_asm_or_system OWNER); des; clarify.
-      + destruct (classic (valid_owner args.(Args.fptr) p)); eauto.
-        right. right. intros SAFE. exploit SAFE; [econs|].
-        i. des.
-        * inv H0.
-        * inv H0. apply H.
-          revert MSFIND st_init INIT. intros MSFIND.
-          ss. rewrite LINK_SK in *.
-          rewrite <- (find_fptr_owner_determ OWNER MSFIND) in *. i.
-          inv INIT. econs; eauto.
-          inv TYP. eauto.
-      + right. left. clarify.
-    - right. right. intros SAFE. clarify. exploit SAFE; [econs|].
+    destruct (classic (exists p, Ge.find_fptr_owner ge args.(Args.fptr) (modsem skenv_link p)
+                                 /\ In (AsmC.module p) prog)) as [[p OWNER] | NOOWNER].
+    - des. simpl_depind.
+      destruct (classic (valid_owner args.(Args.fptr) p)); eauto.
+      right. right. intros SAFE. exploit SAFE; [econs|].
       i. des.
-      + inv H.
-      + inv H. ss. rewrite LINK_SK in *. eauto.
+      + inv H0.
+      + inv H0. apply H.
+        revert MSFIND st_init INIT. intros MSFIND.
+        ss. rewrite LINK_SK in *.
+        rewrite <- (find_fptr_owner_determ OWNER MSFIND) in *. i.
+        inv INIT. econs; eauto.
+        inv TYP. eauto.
+    - destruct (classic (Ge.find_fptr_owner ge fptr (System.modsem skenv_link))).
+      { right. left. esplits; eauto. }
+      right. right. intros SAFE. clarify. exploit SAFE; [econs|].
+      i. des.
+      { inv H0. }
+      inv H0. ss. rewrite LINK_SK in *.
+      destruct (owner_asm_or_system MSFIND); des; clarify.
+      eapply NOOWNER. esplits; et.
   Qed.
 
   Lemma call_step_noevent ge' args frs st1 tr
@@ -1745,6 +1835,7 @@ Section PRESERVATION.
           - i. des. eauto.
         } des.
         econs; cycle 3.
+        * eauto.
         * instantiate (1 := f').
           { inv GEINJECT. econs.
             - i. unfold inject_incr in *.
@@ -1799,7 +1890,7 @@ Section PRESERVATION.
       eapply AsmC.lift_receptive_at.
       eapply semantics_receptive.
       intros EXTERN. eapply not_external in EXTERN; auto.
-      admit "INCL".
+      { eapply ININCL in PROGIN. ss. }
     - econs; i.
       + set (STEP := H). inv STEP. inv H0. eexists. eauto.
       + ii. inv H. ss. omega.
@@ -1820,6 +1911,7 @@ Section PRESERVATION.
           specialize (AGREE PC). rewrite <- FPTR in *.
           inv AGREE. unfold Vnullptr in *. des_ifs. congruence.
         * exploit step_init_simulation; try eassumption.
+          { inv ASMMOD. eauto. }
           i. des. econs 2; ss; eauto. rewrite LINK_SK.
           split; auto. apply star_one. eauto.
       + left. right. econs.
